Add wn ext

theories/semtyping.v
@@ -1,7 +1,7 @@
 Require Import Autosubst2.syntax unscoped par typing.
 Require Import FunctionalExtensionality PropExtensionality.
 From stdpp Require Import relations (rtc(..)).
-Require Import ssreflect.
+Require Import ssreflect ssrbool.
 From Hammer Require Import Tactics.
 From Equations Require Import Equations.
 
@@ -9,6 +9,10 @@ Definition ProdSpace (PA : Tm -> Prop) (PF : Tm -> (Tm -> Prop) -> Prop) (b : Tm
   forall a PB, PA a -> PF a PB -> PB (App b a).
 
 Inductive InterpExt i I : Tm -> (Tm -> Prop) -> Prop :=
+| InterpExt_Ne A :
+  (* ----------------------- *)
+  ne A -> InterpExt i I A wne
+
 | InterpExt_Fun A B PA PF :
   InterpExt i I A PA ->
   (forall a, PA a -> exists PB, PF a PB) ->
@@ -17,10 +21,10 @@ Inductive InterpExt i I : Tm -> (Tm -> Prop) -> Prop :=
 
 | InterpExt_Squash A :
   (* -------------------- *)
-  InterpExt i I (Squash A) (fun a => exists b, rtc Par a (Box b))
+  InterpExt i I (Squash A) (fun a => wne a \/ exists b, rtc Par a (Box b) /\ wn b)
 
 | InterpExt_Empty :
-  InterpExt i I Empty (fun a => False)
+  InterpExt i I Empty wne
 
 | InterpExt_Univ j :
   j < i ->
@@ -52,6 +56,7 @@ Lemma InterpExt_lt_redundant i I0 I1 A PA
        InterpExt i I1 A PA.
 Proof.
   elim : A PA / h.
+  - hauto lq:on ctrs:InterpExt.
   - hauto lq:on ctrs:InterpExt.
   - hauto l:on.
   - hauto l:on ctrs:InterpExt.
@@ -92,6 +97,7 @@ Proof.
   move E : (Pi A B) h => T h.
   move : A B E.
   elim : T P / h => //.
+  - by case.
   - hauto l:on.
   - move => *. subst.
     hauto lq:on rew:off inv:Par ctrs:InterpExt use:Par_subst.
@@ -120,6 +126,76 @@ Lemma InterpUnivN_cumulative i j A PA :
 Proof.
   hauto l:on rew:db:InterpUniv use:InterpExt_cumulative.
 Qed.
+
+Lemma Pars_antirenaming (a b0 : Tm) ξ
+  (h : rtc Par (ren_Tm ξ a) b0) : exists b, b0 = ren_Tm ξ b /\ (rtc Par a b).
+Proof.
+  move E : (ren_Tm ξ a) h => a0 h.
+  move : a E.
+  elim : a0 b0 / h.
+  - hauto lq:on ctrs:rtc.
+  - move => a b c h0 h ih a0 ?. subst.
+    move /Par_antirenaming : h0.
+    hauto lq:on ctrs:rtc, eq.
+Qed.
+
+Lemma wn_antirenaming a ξ : wn (ren_Tm ξ a) -> wn a.
+Proof.
+  hauto lq:on use:Pars_antirenaming, ne_nf_renaming unfold:wn.
+Qed.
+
+Lemma S_Abs a b
+  (h : rtc Par a b) :
+  rtc Par (Abs a) (Abs b).
+Proof. elim : a b /h; hauto lq:on ctrs:Par,rtc. Qed.
+
+Lemma wn_abs (a : Tm) (h : wn a) : wn (Abs a).
+Proof.
+  move : h => [v [? ?]].
+  exists (Abs v).
+  eauto using S_Abs.
+Qed.
+
+Lemma ext_wn i (a : Tm) :
+    wn (App a (VarTm i)) ->
+    wn a.
+Proof.
+  set D := VarTm i.
+  move E : (App a D) => a0 [v [hr hv]].
+  move : hv a E.
+  elim : a0 v /hr.
+  - hauto inv:Tm ctrs:rtc b:on db: nfne.
+  - move => a0 a1 a2 hr0 hr1 ih hnfa2.
+    move /(_ hnfa2) in ih.
+    move => a.
+    case : a0 hr0=>// => b0 b1.
+    elim /Par_inv=>//.
+    + hauto q:on inv:Par ctrs:rtc b:on.
+    + move => ? a0 a3 b2 b3  ? ? [? ?] ? [? ?]. subst.
+      have ? : b3 = D by hauto lq:on inv:Par. subst.
+      suff : wn (Abs a3) by hauto lq:on ctrs:Par, rtc unfold:wn.
+      have : wn (subst_Tm (scons D ids) a3) by sfirstorder.
+      have -> : subst_Tm (scons D ids) a3 = ren_Tm (scons i ids) a3.
+      subst D. substify. by asimpl.
+      move /wn_antirenaming => h.
+      by apply : wn_abs.
+Qed.
+
+Lemma InterpExt_adequacy i I A PA
+  (hI : forall j A,  j < i -> (I j A -> wn A) /\ (wne A -> I j A))
+  (h :  InterpExt i I A PA) :
+  (forall a, PA a -> wn a) /\ (forall a, ne a -> PA a) /\ wn A.
+Proof.
+  set D := VarTm 0.
+  elim : A PA /h.
+  - hauto lq:on use:rtc_refl unfold:wne db:nfne.
+  - move => A B PA PF hPA ihPA hTot hRes ihPF.
+    have hzero : PA D by firstorder.
+    repeat split.
+    + rewrite /ProdSpace => b hb.
+      move /hTot : (hzero) => [PB]hPB.
+
+
 
 Lemma InterpExt_preservation i I A B P (h : ⟦ Ξ ⊨ A ⟧ i ; I ↘ P) :
   (A ⇒ B) ->
